examples/layeredeffects/ID2.fst
@@ -18,7 +18,7 @@ let conjunctive (w:w0 'a) =
   forall p1 p2. w p1 ==> w p2 ==> w (fun x -> p1 x /\ p2 x)
 
 val w (a : Type u#a) : Type u#(max 1 a)
-let w a = w:(w0 a){monotonic w} // /\ conjunctive w}
+let w a = pure_wp a //w:(w0 a){monotonic w} // /\ conjunctive w}
 
 let sat_e (w : w 'a) : Type0 = exists p. w p
 
@@ -29,7 +29,10 @@ let sat (w : w 'a) : Type0 = w (fun _ -> True)
 //          (ensures (w (fun x -> p1 x /\ p2 x)))
 //  = ()
 
-let satlem (w: w 'a) : Lemma (sat_e w <==> sat w) [SMTPat (sat w); SMTPat (sat_e w)] = ()
+open FStar.Monotonic.Pure
+
+let satlem (w: w 'a) : Lemma (sat_e w <==> sat w) [SMTPat (sat w); SMTPat (sat_e w)] =
+  wp_monotonic_pure ()
 
 let repr (a : Type u#aa) (wp : w a) : Type u#aa =
   squash (sat wp) -> v:a{forall p. wp p ==> p v}
@@ -39,19 +42,19 @@ let run (#a:Type) (#w : w a) (c : repr a w{sat w})
   : Tot (v:a{forall p. w p ==> p v})
   = c ()
 
-let test (t : repr int (fun p -> p 42)) =
+let test (t : repr int (coerce_to_pure_wp (fun p -> p 42))) =
   let x1 = run t in
   let x2 = run t in
   assert (x1 == x2)
 
-unfold let return_wp (#a:Type) (x:a) : w a = fun p -> p x
+unfold let return_wp (#a:Type) (x:a) : w a = coerce_to_pure_wp (fun p -> p x)
 
 let return (a : Type) (x : a) : repr a (return_wp x) =
   fun () -> x
 
 unfold let bind_wp (#a:Type) (#b:Type) (wp_f:w a) (wp_g:a -> w b) : w b =
-  let r = fun p -> wp_f (fun x -> wp_g x p) in
-  assert (monotonic r);
+  wp_monotonic_pure ();
+  coerce_to_pure_wp (fun p -> wp_f (fun x -> wp_g x p))
   //let aux (p1 p2 : b->Type0) : Lemma (requires (r p1 /\ r p2))
   //                                 (ensures (r (fun x -> p1 x /\ p2 x))) =
   //  calc (==>) {
@@ -66,7 +69,6 @@ unfold let bind_wp (#a:Type) (#b:Type) (wp_f:w a) (wp_g:a -> w b) : w b =
   //in
   //Classical.forall_intro_2 (fun x y -> Classical.move_requires (aux x) y);
   //assert (conjunctive r);
-  r
 
 let bind (a b : Type) (wp_v : w a) (wp_f: a -> w b)
     (v : repr a wp_v)
@@ -75,7 +77,8 @@ let bind (a b : Type) (wp_v : w a) (wp_f: a -> w b)
  // Fun fact: using () instead of _ below makes us
  // lose the refinement and then this proof fails.
  // Keep that in mind all ye who enter here.
-= fun _ -> f (v ()) () // explicit post is annoying
+= wp_monotonic_pure ();
+  fun _ -> f (v ()) () // explicit post is annoying
 
 let subcomp (a:Type) (wp1 wp2: w a)
     (f : repr a wp1)
@@ -85,7 +88,8 @@ let subcomp (a:Type) (wp1 wp2: w a)
 = f
 
 unfold let if_then_else_wp (#a:Type) (wp1 wp2:w a) (p:bool) : w a =
-  fun post -> (p ==> wp1 post) /\ ((~p) ==> wp2 post)
+  wp_monotonic_pure ();
+  coerce_to_pure_wp (fun post -> (p ==> wp1 post) /\ ((~p) ==> wp2 post))
 
 
 let if_then_else (a : Type) (wp1 wp2 : w a) (f : repr a wp1) (g : repr a wp2) (p : bool) : Type =
@@ -108,33 +112,36 @@ layered_effect {
        if_then_else = if_then_else
 }
 
-let nomon #a (w : w a) : pure_wp a = fun p -> w p
+let nomon #a (w : w a) : pure_wp a =
+  wp_monotonic_pure ();
+  coerce_to_pure_wp (fun p -> w p)
 
 let lift_pure_nd (a:Type) (wp:w a) (f:(eqtype_as_type unit -> PURE a (nomon wp))) :
   Pure (repr a wp) (requires True)
                    (ensures (fun _ -> True))
-  = fun _ -> f ()
+  = wp_monotonic_pure ();
+    fun _ -> f ()
 
 sub_effect PURE ~> ID = lift_pure_nd
 
 
 // this requires using a good if_then_else, but why?
-let rec count (n:nat) : ID int (fun p -> forall r. p r)
+let rec count (n:nat) : ID int (coerce_to_pure_wp (fun p -> forall r. p r))
  = if n = 0 then 0 else count (n-1)
 
 (* Checking that it's kind of usable *)
 
-val test_f : unit -> ID int (fun p -> p 5 /\ p 3)
+val test_f : unit -> ID int (coerce_to_pure_wp (fun p -> p 5 /\ p 3))
 let test_f () = 5
 
 // somehow needs to prove that (forall p. nomon (fun p -> p 5) p) ??
-let test_2 () : ID int (fun p -> p 5) = 5
+let test_2 () : ID int (coerce_to_pure_wp (fun p -> p 5)) = 5
 
 let l () : int =
   reify (test_f ()) ()
 
 effect Id (a:Type) (pre:pure_pre) (post:pure_post' a pre) =
-        ID a (fun (p:pure_post a) -> pre /\ (forall (pure_result:a). post pure_result ==> p pure_result))
+        ID a (coerce_to_pure_wp (fun (p:pure_post a) -> pre /\ (forall (pure_result:a). post pure_result ==> p pure_result)))
 
 effect IdT (a:Type) = Id a True (fun _ -> True)
 
