examples/layeredeffects/ID3.fst
@@ -14,14 +14,15 @@ let w a = pure_wp a
 let repr (a : Type) (wp : w a) : Type =
   v:a{forall p. wp p ==> p v}
 
-unfold
-let return_wp (#a:Type) (x:a) : w a = fun p -> p x
+open FStar.Monotonic.Pure
 
-let return (a : Type) (x : a) : repr a (return_wp x) =
+let return (a : Type) (x : a) : repr a (coerce_to_pure_wp (fun p -> p x)) =
   x
 
 unfold
-let bind_wp (#a #b:Type ) (wp_v:w a) (wp_f:a -> w b) : w b = fun p -> wp_v (fun x -> wp_f x p)
+let bind_wp #a #b (wp_v:w a) (wp_f:a -> w b) : w b =
+  wp_monotonic_pure ();
+  coerce_to_pure_wp (fun p -> wp_v (fun x -> wp_f x p))
 
 let bind (a b : Type) (wp_v : w a) (wp_f: a -> w b)
     (v : repr a wp_v)
@@ -37,7 +38,9 @@ let subcomp (a:Type) (wp1 wp2: w a)
 = f
 
 unfold
-let if_then_else_wp (#a:Type) (wp1 wp2:w a) (p:bool) : w a = fun post -> (p ==> wp1 post) /\ ((~p) ==> wp2 post)
+let if_then_else_wp #a (wp1 wp2:w a) (p:bool) =
+  wp_monotonic_pure ();
+  coerce_to_pure_wp (fun post -> (p ==> wp1 post) /\ ((~p) ==> wp2 post))
 
 let if_then_else (a : Type) (wp1 wp2 : w a) (f : repr a wp1) (g : repr a wp2) (p : bool) : Type =
   repr a (if_then_else_wp wp1 wp2 p)
@@ -62,13 +65,14 @@ layered_effect {
 let lift_pure_nd (a:Type) (wp:pure_wp a) (f:(eqtype_as_type unit -> PURE a wp)) :
   Pure (repr a wp) (requires (wp (fun _ -> True))) // Can only lift from `Tot`
                    (ensures (fun _ -> True))
-  = f ()
+  = wp_monotonic_pure ();
+    f ()
   
 sub_effect PURE ~> ID = lift_pure_nd
 
 (* Checking that it's kind of usable *)
 
-val test_f : unit -> ID int (fun p -> p 5 /\ p 3)
+val test_f : unit -> ID int (coerce_to_pure_wp (fun p -> p 5 /\ p 3))
 let test_f () = 3
 
 module T = FStar.Tactics
@@ -77,12 +81,10 @@ let l () : int =
   reify (test_f ())
 
 effect Id (a:Type) (pre:pure_pre) (post:pure_post' a pre) =
-        ID a (fun (p:pure_post a) -> pre /\ (forall (pure_result:a). post pure_result ==> p pure_result))
+        ID a (coerce_to_pure_wp (fun (p:pure_post a) -> pre /\ (forall (pure_result:a). post pure_result ==> p pure_result)))
 
 effect IdT (a:Type) = Id a True (fun _ -> True)
 
-// Can't lift because of the strengthening, I believe. But can't we
-// prove it on the spot?
 let rec sum (l : list int) : IdT int
  =
   match l with
