examples/layeredeffects/IteSoundness.fst
@@ -38,13 +38,16 @@ irreducible let an_attr : unit = ()
 
 type repr (a:Type) (wp:pure_wp a) = unit -> PURE a wp
 
+open FStar.Monotonic.Pure
+
 unfold
-let return_wp (#a:Type) (x:a) = fun p -> p x
+let return_wp (#a:Type) (x:a) : pure_wp a = coerce_to_pure_wp (fun p -> p x)
 let return (a:Type) (x:a) : repr a (return_wp x) = fun () -> x
 
 unfold
 let bind_wp (#a #b:Type) (wp1:pure_wp a) (wp2:a -> pure_wp b) : pure_wp b =
-  fun p -> wp1 (fun x -> wp2 x p)
+  wp_monotonic_pure ();
+  coerce_to_pure_wp (fun p -> wp1 (fun x -> wp2 x p))
 let bind (a b:Type) (wp1:pure_wp a) (wp2:a -> pure_wp b)
   (f:repr a wp1)
   (g:(x:a -> repr b (wp2 x)))
@@ -61,12 +64,13 @@ let subcomp (a:Type) (wp1 wp2:pure_wp a) (f:repr a wp1)
   = f
 
 unfold
-let ite_wp (#a:Type) (wp_then wp_else:pure_wp a) (b:bool) : Type =
-  repr a (fun p -> (b ==> wp_then p) /\ ((~ b) ==> wp_else p))
+let ite_wp (#a:Type) (wp_then wp_else:pure_wp a) (b:bool) : pure_wp a =
+  wp_monotonic_pure ();
+  coerce_to_pure_wp (fun p -> (b ==> wp_then p) /\ ((~ b) ==> wp_else p))
 let if_then_else (a:Type) (wp_then wp_else:pure_wp a)
   (f:repr a wp_then) (g:repr a wp_else)
   (b:bool)
-  : Type = ite_wp wp_then wp_else b
+  : Type = repr a (ite_wp wp_then wp_else b)
 
 (*
  * The tactic that will solve the implicits and guard for if-then-else soundness
